theories/gitree/reify.v
@@ -2,70 +2,634 @@ From iris.proofmode Require Import classes tactics.
 From gitrees Require Import prelude.
 From gitrees.gitree Require Import core.
 
+Section abstract_res.
+  Variable (R : Type).
+  Variable (Op : R → Type).
+  Variable (In : forall {r : R}, Op r → oFunctor).
+  Variable (Out : forall {r : R}, Op r → oFunctor).
+  Variable (St : R → oFunctor).
+
+  Definition reifier_type (r : R) : Type :=
+    forall (op : Op r) {X} `{!Cofe X},
+      ((In op ♯ X) * (St r ♯ X) -n> (Out op ♯ X) * (St r ♯ X))%type.
+
+  Variable (Re : forall r, reifier_type r).
+
+  Inductive hvec : nat → Type :=
+  | nil : hvec 0
+  | cons {n} : R → hvec n → hvec (S n).
+
+  Definition hvec_S_inv {n} (P : hvec (S n) → Type)
+    (Hcons : ∀ sR v, P (cons sR v)) v : P v.
+  Proof.
+    revert P Hcons.
+    refine match v with nil => tt
+                      | cons sR v => λ P Hcons, Hcons sR v end.
+  Defined.
+
+  Global Instance hvec_lookup_total : ∀ m, LookupTotal (fin m) R (hvec m) :=
+  fix go m i {struct i} := let _ : ∀ m, LookupTotal _ _ _ := @go in
+  match i in fin m return hvec m → R with
+  | 0%fin => hvec_S_inv (λ _, R) (λ x _, x)
+  | FS j => hvec_S_inv (λ _, R) (λ _ v, v !!! j)
+  end.
+
+  (** global signature *)
+  Definition glob_Op {n} (rs : hvec n) : Type :=
+    { i : fin n & Op (rs !!! i) }.
+  Definition glob_In {n} {rs : hvec n} : glob_Op rs → oFunctor :=
+    λ iop, @In (rs !!! projT1 iop) (projT2 iop).
+  Definition glob_Out {n} {rs : hvec n} : glob_Op rs → oFunctor :=
+    λ iop, @Out (rs !!! projT1 iop) (projT2 iop).
+
+  Fixpoint glob_St {n} (rs : hvec n) : oFunctor :=
+    match rs with
+    | nil => unitO
+    | cons r rs => St r * glob_St rs
+    end%OF.
+
+  Fixpoint glob_St_rest {n} (i : fin n) : hvec n → oFunctor :=
+    match i in fin n return hvec n → oFunctor with
+    | 0%fin => hvec_S_inv (λ _, oFunctor)
+                 (λ _ rs, glob_St rs)
+    | FS j => hvec_S_inv (λ _, oFunctor)
+                 (λ r rs, St r * glob_St_rest j rs)%OF
+    end.
+
+  Lemma glob_St_decomp' {m} (i : fin m) (rs : hvec m) {X} `{!Cofe X} :
+    ofe_iso (glob_St rs ♯ X) ((St (rs !!! i) ♯ X) * (glob_St_rest i rs ♯ X))%type.
+  Proof.
+    revert i. induction rs as [|n r rs]=>i.
+    { inversion i. }
+    inv_fin i; simpl.
+    { apply iso_ofe_refl. }
+    intros i.
+    specialize (IHrs i).
+    unshelve esplit.
+    - simple refine (λne xr, let sr := ofe_iso_1 IHrs (xr.2) in
+                             (sr.1,(xr.1,sr.2))).
+      solve_proper.
+    - simple refine (λne sxr, let r' := ofe_iso_2 IHrs (sxr.1,sxr.2.2) in
+                              (sxr.2.1, r')).
+      solve_proper.
+    - intros (s & x & rest). simpl. repeat f_equiv; rewrite ofe_iso_12//.
+    - intros (x & rest). simpl. f_equiv.
+      rewrite -surjective_pairing. apply ofe_iso_21.
+  Qed.
+  Definition glob_St_decomp {m} (i : fin m) {rs : hvec m} {X} `{!Cofe X} :
+    (glob_St rs ♯ X) -n> ((St (rs !!! i) ♯ X) * (glob_St_rest i rs ♯ X))%type
+    := ofe_iso_1 (glob_St_decomp' i rs).
+  Program Definition glob_St_recomp {m} {i : fin m} {rs : hvec m} {X} `{!Cofe X} :
+    (glob_St_rest i rs ♯ X) -n> (St (rs !!! i) ♯ X) -n> (glob_St rs ♯ X)
+    := λne rest st, ofe_iso_2 (glob_St_decomp' i rs) (st, rest).
+  Solve All Obligations with solve_proper_please.
+
+  Lemma glob_St_decomp_recomp {m} (i : fin m) {rs : hvec m} {X} `{!Cofe X}
+    (σ : St (rs !!! i) ♯ X) rest :
+    glob_St_decomp i (glob_St_recomp rest σ) ≡ (σ, rest).
+  Proof. rewrite ofe_iso_12. reflexivity. Qed.
+
+  Definition glob_Re {n} {rs : hvec n} (op : glob_Op rs) {X} `{!Cofe X} :
+    (glob_In op ♯ X) * (glob_St rs ♯ X) → (glob_Out op ♯ X) * (glob_St rs ♯ X)
+    :=  λ xst,
+      let  i := projT1 op in
+      let op' := projT2 op in
+      let x := xst.1 in
+      let st := xst.2 in
+      let fs := glob_St_decomp i st in
+      let σ := fs.1 in
+      let rest := fs.2 in
+      let rx := Re (rs !!! i) op' _ _ (x, σ) in
+      (rx.1, glob_St_recomp rest rx.2).
+
+  Record in_hvec {n} (r : R) (rs : hvec n) : Type :=
+    { idx : fin n;
+      opF : Op r → Op (rs !!! idx);
+      inF {X} `{!Cofe X} (op : Op r) :
+        ofe_iso (In op ♯ X) (In (opF op) ♯ X);
+      outF {X} `{!Cofe X} (op : Op r) :
+        ofe_iso (Out op ♯ X) (Out (opF op) ♯ X);
+      stF  {X} `{!Cofe X} :
+        ofe_iso (St r ♯ X) (St (rs !!! idx) ♯ X);
+      reF {X} `{!Cofe X} (op : Op r) (x : In op ♯ X)
+          (y : Out op ♯ X) (s1 s2 : St r ♯ X) :
+        Re r op X _ (x, s1) ≡ (y, s2) →
+          Re (rs !!! idx) (opF op) X _ (ofe_iso_1 (inF op) x, ofe_iso_1 stF s1) ≡
+            (ofe_iso_1 (outF op) y, ofe_iso_1 stF s2)
+    }.
+  Arguments idx {_ _ _} _.
+
+  Definition in_hvec_op {n} {r : R} {rs : hvec n} (rin : in_hvec r rs)
+    (op : Op r) : glob_Op rs.
+  Proof.
+    refine (existT (idx rin) _).
+    apply (opF _ _ rin op).
+  Defined.
+  Definition in_hvec_in {n} {r : R} {rs : hvec n} (rin : in_hvec r rs)
+                        {X} `{Cofe X} (op : Op r)
+    (x : In op ♯ X) : glob_In (in_hvec_op rin op) ♯ X.
+  Proof.
+    unfold glob_In.
+    unfold in_hvec_op; simpl.
+    apply (ofe_iso_1 (inF _ _ _ _) x).
+  Defined.
+  Definition in_hvec_st {n} {r : R} {rs : hvec n} (rin : in_hvec r rs)
+                        {X} `{Cofe X} (op : Op r)
+    (x : St r ♯ X) : St (rs !!! idx rin) ♯ X.
+  Proof.
+    apply (ofe_iso_1 (stF _ _ _) x).
+  Defined.
+  Definition in_hvec_out {n} {r : R} {rs : hvec n} (rout : in_hvec r rs)
+                        {X} `{Cofe X} (op : Op r)
+    (x : Out op ♯ X) : glob_Out (in_hvec_op rout op) ♯ X.
+  Proof.
+    unfold glob_Out.
+    unfold in_hvec_op; simpl.
+    apply (ofe_iso_1 (outF _ _ _ _) x).
+  Defined.
+
+  Lemma glob_Re_idx {n} (r : R) (rs : hvec n) (rin : in_hvec r rs)
+    {X} `{!Cofe X} (i : fin n) (op : Op (rs !!! i))
+    (x : In op ♯ X) (σ : St (rs !!! i) ♯ X) (rest : glob_St_rest i rs ♯ X) :
+    glob_Re (existT i op) (x,glob_St_recomp rest σ) ≡
+      prodO_map idfun (glob_St_recomp rest) $ Re (rs !!! i) op X _ (x,σ).
+  Proof.
+    Opaque glob_St_recomp.
+    unfold glob_Re. simpl.
+    trans (((Re (rs !!! i) op X _ (x, σ)).1, glob_St_recomp rest (Re (rs !!! i) op X _ (x, σ)).2)).
+    { repeat f_equiv; rewrite glob_St_decomp_recomp//. }
+    destruct (Re (rs !!! i) op X _ (x, σ)) as [y σ'].
+    simpl. reflexivity.
+  Qed.
+
+  Lemma in_hvec_re {n} (r : R) (rs : hvec n) (rin : in_hvec r rs)
+                   {X} `{!Cofe X}
+                   (op : Op r) (x : In op ♯ X) (σ : St r ♯ X)
+                   (y : Out op ♯ X) (σ' : St r ♯ X)
+                   (rest : glob_St_rest (idx rin) rs ♯ X)
+    : Re r op X _ (x,σ) ≡ (y, σ') →
+      glob_Re (in_hvec_op rin op)
+        (in_hvec_in rin _ x,glob_St_recomp rest (in_hvec_st rin op σ))
+        ≡ (in_hvec_out rin _ y, glob_St_recomp rest (in_hvec_st rin op σ')).
+  Proof.
+    intros Hre.
+    apply (reF r rs rin) in Hre.
+    unfold in_hvec_op.
+    rewrite glob_Re_idx//.
+    rewrite Hre. simpl. reflexivity.
+  Qed.
+
+End abstract_reseeee.
+
+
 Section reify.
   Definition reify_eff (E : opsInterp) (stateF : oFunctor) :=
     ∀ (op : opid E) (X : ofe) `{Cofe X},
-    ((Ins (E op) ♯ X) * (stateF ♯ X) -n> optionO ((Outs (E op) ♯ X) * (stateF ♯ X)))%type.
+      ((Ins (E op) ♯ X) * (stateF ♯ X) -n> optionO ((Outs (E op) ♯ X) * (stateF ♯ X)))%type.
 
-  Inductive reifiers : opsInterp → Type :=
-  | reifiers_nil : reifiers @[]
-  | reifiers_cons
-      (E : opsInterp) (stateF : oFunctor) (re : reify_eff E stateF)
-      {Hinh : Inhabited (stateF ♯ unitO)}
-      {Hcofe : forall X (HX : Cofe X), Cofe (stateF ♯ X)}
-      {E'} (tail : reifiers E') : reifiers (opsInterp.app E E').
+  Record sReifier :=
+    { sReifier_ops : opsInterp;
+      sReifier_state : oFunctor;
+      sReifier_re : reify_eff sReifier_ops sReifier_state;
+      sReifier_inhab :: Inhabited (sReifier_state ♯ unitO);
+      sReifier_cofe X (HX : Cofe X) :: Cofe (sReifier_state ♯ X);
+    }.
+  Set Printing Universes.
+  About list. About Vector.t.
+  Coercion  sReifier_re : sReifier >-> Funclass.
 
-  Fixpoint reifiers_state {E} (rs : reifiers E) : oFunctor :=
+  Inductive gReifiers : nat → Type :=
+  | gReifiers_nil : gReifiers 0
+  | gReifiers_cons {n} : sReifier → gReifiers n → gReifiers (S n)
+  .
+
+  Fixpoint gReifiers_state {n} (rs : gReifiers n) : oFunctor :=
     match rs with
-    | reifiers_nil => unitO
-    | reifiers_cons _ stateF _ tail => stateF * (reifiers_state tail)
+    | gReifiers_nil => unitO
+    | gReifiers_cons sR rs => sReifier_state sR * (gReifiers_state rs)
     end.
 
-  #[export] Instance reifiers_state_cofe E (rs : reifiers E) X `{!Cofe X} :
-    Cofe (reifiers_state rs ♯ X).
-  Proof. induction rs; simpl; apply _. Qed.
-  #[export] Instance reifiers_state_inhab E (rs : reifiers E) :
-    Inhabited (reifiers_state rs ♯ unitO).
-  Proof. induction rs; simpl; apply _. Qed.
+  Fixpoint gReifiers_ops {n} (rs : gReifiers n) : opsInterp :=
+    match rs with
+    | gReifiers_nil => opsInterp.nil
+    | gReifiers_cons sR rs => opsInterp.app (sReifier_ops sR) (gReifiers_ops rs)
+    end.
 
-
-  Definition reifiers_re {E} (rs : reifiers E) (op : opid E) (X : ofe) `{Cofe X} :
-    ((Ins (E op) ♯ X) * (reifiers_state rs ♯ X) → optionO ((Outs (E op) ♯ X) * (reifiers_state rs ♯ X)))%type.
+  Definition grs_S_inv {n} (P : gReifiers (S n) → Type)
+    (Hcons : ∀ sR v, P (gReifiers_cons sR v)) v : P v.
   Proof.
-    revert op. induction rs=>op.
-    { apply Empty_set_rect. exact op. }
-    simpl reifiers_state.
-    destruct op as [op|op]; simpl.
-    - refine (λ '(i,(s,s_rest)),
-               '(o,s') ← re op X _ (i, s);
-               Some (o,(s',s_rest))).
-    - refine (λ '(i,(s,s_rest)),
-               '(o,s'_rest) ← IHrs op (i,s_rest);
-               Some (o,(s,s'_rest))
-             ).
+    revert P Hcons.
+    refine match v with gReifiers_nil => tt
+                      | gReifiers_cons sR v => λ P Hcons, Hcons sR v end.
   Defined.
 
-  #[global] Instance reifiers_re_ne {E} (rs : reifiers E) (op : opid E) (X : ofe) `{Cofe X} :
+  Global Instance gReifiers_lookup_total : ∀ m, LookupTotal (fin m) sReifier (gReifiers m) :=
+  fix go m i {struct i} := let _ : ∀ m, LookupTotal _ _ _ := @go in
+  match i in fin m return gReifiers m → sReifier with
+  | 0%fin => grs_S_inv (λ _, sReifier) (λ x _, x)
+  | FS j => grs_S_inv (λ _, sReifier) (λ _ v, v !!! j)
+  end.
+
+  Fixpoint gReifiers_state_rest {m} (i : fin m) : gReifiers m → oFunctor :=
+    match i in fin m return gReifiers m → oFunctor with
+    | 0%fin => grs_S_inv (λ _, oFunctor)
+                 (λ sR rs, gReifiers_state rs)
+    | FS j => grs_S_inv (λ _, oFunctor)
+                 (λ sR rs, sReifier_state sR * gReifiers_state_rest j rs)%OF
+    end.
+
+  Lemma rs_state_decomp {m} (i : fin m) (rs : gReifiers m) {X} `{!Cofe X} :
+    ofe_iso ((sReifier_state (rs !!! i) ♯ X) * (gReifiers_state_rest i rs ♯ X))%type
+            (gReifiers_state rs ♯ X).
+  Proof.
+    revert i. induction rs as [|? [F stateF re ? ?] rs]=>i.
+    { inversion i. }
+    inv_fin i; simpl.
+    { apply iso_ofe_refl. }
+    intros i.
+    specialize (IHrs i).
+    unshelve esplit.
+    - simple refine (λne sxr, let r' := ofe_iso_1 IHrs (sxr.1,sxr.2.2) in
+                              (sxr.2.1, r')).
+      solve_proper.
+    - simple refine (λne xr, let sr := ofe_iso_2 IHrs (xr.2) in
+                             (sr.1,(xr.1,sr.2))).
+      solve_proper.
+    - intros (x & r). simpl. f_equiv.
+      rewrite -surjective_pairing. apply ofe_iso_12.
+    - intros (s & x & r). simpl. repeat f_equiv; rewrite ofe_iso_21//.
+  Qed.
+
+  #[export] Instance reifiers_state_cofe {n} (rs : gReifiers n) X `{!Cofe X} :
+    Cofe (gReifiers_state rs ♯ X).
+  Proof.
+    induction rs; simpl; first apply _.    destruct s. apply _.
+  Qed.
+  #[export] Instance reifiers_state_inhab {n} (rs : gReifiers n) :
+    Inhabited (gReifiers_state rs ♯ unitO).
+  Proof.
+    induction rs; simpl; first apply _.
+    destruct s. apply _.
+  Qed.
+
+  Definition reifiers_op_idx' {n} (rs : gReifiers n)
+    (op : opid (gReifiers_ops rs)) :
+    { i : fin n & opid (sReifier_ops (rs !!! i)) }.
+  Proof.
+    induction rs as [|? sR rs].
+    { apply Empty_set_rect. exact op. }
+    simpl in op.
+    destruct op as [op|op]; simpl.
+    - refine (existT 0%fin op).
+    - pose (i := projT1 (IHrs op)).
+      exact (existT (FS i) (projT2 (IHrs op))).
+  Defined.
+  Definition reifiers_op_idx {n} (rs : gReifiers n)
+    (op : opid (gReifiers_ops rs)) : fin n
+    := projT1 $ reifiers_op_idx' rs op.
+  Definition reifiers_op_conv {n} (rs : gReifiers n)
+    (op : opid (gReifiers_ops rs)) : opid (sReifier_ops (rs !!! reifiers_op_idx rs op))
+    := projT2 $ reifiers_op_idx' rs op.
+  Lemma reifiers_op_idx_0 {n} (sR : sReifier) (rs : gReifiers n)
+    (op : opid (sReifier_ops sR)) :
+    reifiers_op_idx (gReifiers_cons sR rs) (inl op) = 0%fin.
+  Proof. reflexivity. Qed.
+  Lemma reifiers_op_idx_S {n} (sR : sReifier) (rs : gReifiers n)
+    (op : opid (gReifiers_ops rs)) :
+    reifiers_op_idx (gReifiers_cons sR rs) (inr op) = FS $ reifiers_op_idx rs op.
+  Proof. reflexivity. Qed.
+
+  (* those are just identities? *)
+  Definition reifiers_op_conv_ins {n} (rs : gReifiers n)
+    (op : opid (gReifiers_ops rs)) {X} `{!Cofe X}:
+    ofe_iso (Ins (gReifiers_ops rs op) ♯ X)
+      (Ins (sReifier_ops (rs !!! (reifiers_op_idx rs op)) (reifiers_op_conv rs op)) ♯ X).
+  Proof.
+    induction rs as [|? [F stateF re ? ?] rs].
+    { apply Empty_set_rect. exact op. }
+    simpl in op.
+    destruct op as [op|op].
+    - unfold reifiers_op_conv. simpl.
+      apply iso_ofe_refl.
+    - simpl. unfold reifiers_op_conv.
+      apply IHrs.
+  Defined.
+  Definition reifiers_op_conv_outs {n} (rs : gReifiers n)
+    (op : opid (gReifiers_ops rs)) {X} `{!Cofe X}:
+    ofe_iso (Outs (gReifiers_ops rs op) ♯ X)
+      (Outs (sReifier_ops (rs !!! (reifiers_op_idx rs op)) (reifiers_op_conv rs op)) ♯ X).
+  Proof.
+    induction rs as [|? [F stateF re ? ?] rs].
+    { apply Empty_set_rect. exact op. }
+    simpl in op.
+    destruct op as [op|op].
+    - unfold reifiers_op_conv. simpl.
+      apply iso_ofe_refl.
+    - simpl. unfold reifiers_op_conv.
+      apply IHrs.
+  Defined.
+
+  Program Definition reifiers_op_conv_state {n} {i : fin n} {rs : gReifiers n}
+   {X} `{!Cofe X} :
+    (rs_state_rest i rs ♯ X) -n>
+    (sReifier_state (rs !!! i) ♯ X) -n>
+      gReifiers_state rs ♯ X :=
+    λne rest σ1,  ofe_iso_1 (rs_state_decomp i rs) (σ1,rest).
+  Solve All Obligations with solve_proper_please.
+
+  Program Definition reifiers_op_conv_state' {n} (i : fin n) {rs : gReifiers n}
+    {X} `{!Cofe X} :
+    gReifiers_state rs ♯ X -n>
+      (prodO (sReifier_state (rs !!! i) ♯ X) (rs_state_rest i rs ♯ X))
+    := ofe_iso_2 (rs_state_decomp i rs).
+
+  Definition reifiers_re_idx {n} (i : fin n) (rs : gReifiers n)
+    (op : opid (sReifier_ops (rs !!! i))) (X : ofe) `{Cofe X} :
+    ((Ins (sReifier_ops (rs !!! i) op) ♯ X) * (gReifiers_state rs ♯ X)
+     → optionO ((Outs (sReifier_ops (rs !!! i) op) ♯ X) * (gReifiers_state rs ♯ X)))%type.
+  Proof.
+    intros [inp s].
+    set (σ := fst (reifiers_op_conv_state' i s)).
+    set (rest := snd (reifiers_op_conv_state' i s)).
+    simple refine (optionO_map (prodO_map idfun (reifiers_op_conv_state rest)) (sReifier_re (rs !!! i) op X _ (inp, σ))).
+  Defined.
+
+  #[global] Instance reifiers_re_idx_ne  {n} (i : fin n) (rs : gReifiers n)
+    (op : opid (sReifier_ops (rs !!! i))) (X : ofe) `{Cofe X} :
+    NonExpansive (reifiers_re_idx i rs op X).
+  Proof.
+    intros m [i1 s1] [i2 s2] [Hi Hs].
+    unfold reifiers_re_idx. repeat f_equiv; eauto.
+  Qed.
+
+  (* Definition reifiers_re {n} (rs : gReifiers n) *)
+  (*   (op : opid (gReifiers_ops rs)) (X : ofe) `{Cofe X} : *)
+  (*   ((Ins (gReifiers_ops rs op) ♯ X) * (gReifiers_state rs ♯ X) *)
+  (*    → optionO ((Outs (gReifiers_ops rs op) ♯ X) * (gReifiers_state rs ♯ X)))%type. *)
+  (* Proof. *)
+  (*   intros xs. *)
+  (*   refine *)
+  (*     (optionO_map (prodO_map (ofe_iso_2 (reifiers_op_conv_outs rs op)) idfun) $ reifiers_re_idx (reifiers_op_idx rs op) rs (reifiers_op_conv rs op) X *)
+  (*        (ofe_iso_1 (reifiers_op_conv_ins rs op) xs.1, xs.2)). *)
+  (* Defined. *)
+  Definition reifiers_re {n} (rs : gReifiers n)
+    (op : opid (gReifiers_ops rs)) (X : ofe) `{Cofe X} :
+    ((Ins (gReifiers_ops rs op) ♯ X) * (gReifiers_state rs ♯ X)
+     → optionO ((Outs (gReifiers_ops rs op) ♯ X) * (gReifiers_state rs ♯ X)))%type.
+  Proof.
+    induction rs as [|? sR rs].
+    { inversion op. }
+    simpl in op.
+    destruct op as [op|op]; cbn-[oFunctor_apply].
+    - intros [x [s1 s2]].
+      apply (option_map (prod_map idfun (λ s1', (s1',s2))) (sReifier_re sR op X _ (x,s1))).
+    - intros [x [s1 s2]].
+      apply
+        (option_map (prod_map idfun (λ s2', (s1,s2'))) (IHrs _ (x,s2))).
+  Defined.
+
+
+  #[global] Instance reifiers_re_ne {n} (rs : gReifiers n)
+       (op : opid (gReifiers_ops rs)) (X : ofe) `{Cofe X} :
     NonExpansive (reifiers_re rs op X).
   Proof.
-    induction rs; simpl.
-    { apply Empty_set_rect. exact op. }
-    destruct op as [op|op]; simpl.
-    - intros n [x1 [s1 s1_rst]]  [x2 [s2 s2_rst]] [Hx [Hs Hsrest]].
-      apply option_mbind_ne; last solve_proper.
-      intros [o1 s'1] [o2 s'2] [Ho Hs']. solve_proper.
-    - intros n [x1 [s1 s1_rst]]  [x2 [s2 s2_rst]] [Hx [Hs Hsrest]].
-      apply option_mbind_ne; last solve_proper.
-      intros [o1 s'1] [o2 s'2] [Ho Hs']. solve_proper.
-  Qed.
-  #[global] Instance reifiers_re_proper {E} (rs : reifiers E) (op : opid E) (X : ofe) `{Cofe X} :
+    (* unfold reifiers_re. solve_proper_please. *)
+  Admitted.
+  #[global] Instance reifiers_re_proper  {n} (rs : gReifiers n)
+       (op : opid (gReifiers_ops rs)) (X : ofe) `{Cofe X} :
     Proper ((≡) ==> (≡)) (reifiers_re rs op X).
   Proof. apply ne_proper. apply _. Qed.
 
-  Variable (E : opsInterp) (rs : reifiers E).
-  Notation IT := (IT E).
-  Notation ITV := (ITV E).
-  Notation stateF := (reifiers_state rs).
+  (* Class inReifier {n} (sR : sReifier) (rs : gReifiers n) := *)
+  (*   { inR_idx : fin n; *)
+  (*     inR_lookup : rs !!! inR_idx = sR *)
+  (*   }. *)
+  Class inReifier {n} (sR : sReifier) (rs : gReifiers n) :=
+    { inR_idx : fin n;
+      inR_sub :: subEff (sReifier_ops sR) (sReifier_ops (rs !!! inR_idx));
+      inR_state X `{!Cofe X} :
+         ofe_iso (sReifier_state sR ♯ X)
+                 (sReifier_state (rs !!! inR_idx) ♯ X);
+      inR_reify X `{!Cofe X} (op : opid (sReifier_ops sR))
+          (x : Ins (sReifier_ops sR op) ♯ X)
+          (s : sReifier_state sR ♯ X) :
+      let x' : Ins (sReifier_ops (rs !!! inR_idx) (subEff_opid op)) ♯ X
+        := subEff_conv_ins x in
+      let s' : sReifier_state (rs !!! inR_idx) ♯ X
+        := ofe_iso_1 (inR_state X) s in
+         sReifier_re sR op X _ (x , s) ≡
+         optionO_map (prodO_map subEff_conv_outs2 (ofe_iso_2 (inR_state X))) $
+           sReifier_re (rs !!! inR_idx) (subEff_opid op) X _ (x', s')
+    }.
+  Definition inReifier_st_conv {n} {sR} {rs : gReifiers n} `{!inReifier sR rs}
+    {X} `{!Cofe X}:
+    sReifier_state sR ♯ X -n> sReifier_state (rs !!! inR_idx) ♯ X
+    := ofe_iso_1 (inR_state X).
+  Definition inReifier_st_conv2 {n} {sR} {rs : gReifiers n} `{!inReifier sR rs}
+    {X} `{!Cofe X}:
+    sReifier_state (rs !!! inR_idx) ♯ X -n> sReifier_state sR ♯ X
+    := ofe_iso_2 (inR_state X).
+
+  (* Program Definition sRs_transport {A B : sReifier} (H : A = B) *)
+  (*   {X} `{!Cofe X} : *)
+  (*   ofe_iso (sReifier_state A ♯ X) (sReifier_state B ♯ X) *)
+  (*   := eq_rect A (λ B, ofe_iso (sReifier_state B ♯ X) (sReifier_state B ♯ X)) *)
+  (*        iso_ofe_refl B H. *)
+  (* Next Obligation. solve_proper. Qed. *)
+
+  (* Definition sReq_opid {A B : sReifier} (H : A = B) : *)
+  (*   opid (sReifier_ops A) = opid (sReifier_ops B). *)
+  (* Proof. *)
+  (*   induction H. reflexivity. *)
+  (* Defined. *)
+  (* Definition sRop_transport {A B : sReifier} (H : A = B) : *)
+  (*   opid (sReifier_ops A) → opid (sReifier_ops B). *)
+  (* Proof. *)
+  (*   induction H. exact id. *)
+  (* Defined. *)
+
+  (* Definition inR_opid {n} {sR} (rs : gReifiers n) {i : fin n} *)
+  (*   (Hi : rs !!! i = sR): *)
+  (*   opid (sReifier_ops sR) → opid (gReifiers_ops rs). *)
+  (* Proof. *)
+  (*   induction rs as [|? sR' rs]. *)
+  (*   { inversion i. } *)
+  (*   inv_fin i. *)
+  (*   { simpl. intros Hsr. *)
+  (*     refine (inl ∘ sRop_transport (eq_sym Hsr)). } *)
+  (*   intros i. simpl. intros Hi. *)
+  (*   refine (inr ∘ IHrs i Hi). *)
+  (* Defined. *)
+
+  (* Definition subEff_transp {sR sR'} (H : sR = sR') : *)
+  (*   subEff (sReifier_ops sR) (sReifier_ops sR'). *)
+  (* Proof. *)
+  (*   refine {| subEff_opid := sRop_transport H |}. *)
+  (*   - intros. *)
+  (*     assert ((sReifier_ops sR op) = (sReifier_ops sR' (sRop_transport H op))). *)
+  (*     { *)
+  (*       rewrite sReq_opid. *)
+  (*     intros op X HX. *)
+  #[global] Instance inR_subEff' {n} (i : fin n) (rs : gReifiers n) :
+    subEff (sReifier_ops (rs !!! i)) (gReifiers_ops rs).
+  Proof.
+    induction rs as [|? sR' rs].
+    { inversion i. }
+    inv_fin i.
+    { simpl. apply _. }
+    intros i. simpl.
+    apply subEff_app_r.
+    apply IHrs.
+  Defined.
+
+  Definition subEff_comp E1 E2 E3 :
+    subEff E1 E2 → subEff E2 E3 → subEff E1 E3.
+  Proof.
+    intros H1 H2.
+    simple refine
+             {| subEff_opid (op : opid E1) := subEff_opid (subEff_opid op) |}.
+    - intros.
+      eapply iso_ofe_trans.
+      + apply subEff_ins.
+      + apply subEff_ins.
+    - intros.
+      eapply iso_ofe_trans.
+      + apply subEff_outs.
+      + apply subEff_outs.
+  Defined.
+
+  #[global] Instance inR_subEff {n} sR (rs : gReifiers n) :
+    inReifier sR rs → subEff (sReifier_ops sR) (gReifiers_ops rs).
+  Proof.
+    intros HR.
+    eapply subEff_comp.
+    - apply HR.
+    - apply inR_subEff'.
+  Defined.
+
+  Global Instance optionO_map_proper A B f :
+    Proper ((≡) ==> (≡)) (@optionO_map A B f).
+  Proof. apply ne_proper. apply _. Qed.
+
+
+  (* XXX: see why sReifier_re does not work as a good coercion here *)
+  Lemma inR_subreify {n} sR (rs : gReifiers n)
+   {inR0 : inReifier sR rs}
+    {X} `{!Cofe X}
+    (σ : sReifier_state sR ♯ X)
+    (rest : rs_state_rest inR_idx rs ♯ X)
+    (op : opid (sReifier_ops sR))
+    (i : Ins (sReifier_ops sR op) ♯ X)
+    :
+    let σ1 := inReifier_st_conv σ in
+    let fs1 := reifiers_op_conv_state rest σ1 in
+    reifiers_re rs (subEff_opid op) X (ofe_iso_1 (subEff_ins op) i, fs1) ≡
+     optionO_map (prodO_map subEff_conv_outs (reifiers_op_conv_state rest ◎ inReifier_st_conv))
+      (sReifier_re sR op X _ (i, σ)).
+  Proof.
+    intros σ1.
+    set (i' := subEff_conv_ins i).
+    intros fs1.
+    assert (sReifier_re sR op X _ (i,σ) ≡
+       optionO_map (prodO_map subEff_conv_outs2 inReifier_st_conv2)
+       (sReifier_re (rs !!! inR_idx) (subEff_opid op) X _ (i', σ1))) as Heq.
+    { apply inR_reify. }
+    pose (op1 :=  (@subEff_opid (sReifier_ops sR) (sReifier_ops (rs !!! @inR_idx n sR rs inR0))) inR_sub op).
+    fold op1 in Heq.
+    pose  (op' := @subEff_opid _ (@gReifiers_ops n rs)
+                    (@inR_subEff' n _ rs) op1).
+    change (@subEff_opid (sReifier_ops sR) (@gReifiers_ops n rs) (@inR_subEff n sR rs inR0) op) with op'.
+    induction rs as [|? sR' rs].
+    { pose (j:= inR_idx). inversion j. }
+    simpl in op'. 
+    remember op' as op2.
+    Set Printing All.
+    Etrans. 2:{
+            apply optionO_map_proper.
+            symmetry. apply Heq. }
+          unfold reifiers_re. simpl fst. simpl snd.
+    pose (op1 :=  (@subEff_opid (sReifier_ops sR) (sReifier_ops (rs !!! @inR_idx n sR rs inR0))) inR_sub op).
+    fold op1.
+    pose  (op' := @subEff_opid _ (@gReifiers_ops n rs)
+                    (@inR_subEff' n _ rs) op1).
+Set Printing Implicit.
+    fold op'.
+    induction rs as [|? sR' rs].
+    { pose (j:= inR_idx). inversion j. }
+    simpl in op'.
+    destruct op' as [op'|op'].
+    simpl reifiers_op_idx.
+    simpl.
+    unfold reifiers_re. simpl.
+    
+    set ().
+    set (| 
+    Check .
+    
+    : let σ1 := ofe_iso_2 (sRs_transport inR_lookup) σ in
+      let fs1 := reifiers_op_conv_state rest σ1 in
+   reifiers_re rs (subEff_opid op) X (ofe_iso_1 (subEff_ins op) i, fs1) ≡
+   optionO_map (prodO_map (ofe_iso_1 (subEff_outs op)) (reifiers_op_conv_state rest ◎ ofe_iso_2 (sRs_transport inR_lookup)))
+     (sReifier_re sR op X _ (i, σ)).
+  Proof.
+    revert op i σ rest.
+    induction rs as [|? sR' rs]=>op i σ rest.
+    { destruct inR0.
+      inversion inR_idx0. }
+    pose (HH := inR_subEff _ _ inR0).
+    destruct inR0.
+    inv_fin inR_idx0.
+    { intros Heq rest HH.
+      simpl in Heq.
+      unfold reifiers_re.
+      Set Printing Implicit.
+      simpl subEff_opid.
+      assert (reifiers_op_idx rs op)
+      simpl.
+      generalize (@subEff_opid (sReifier_ops sR) (@gReifiers_ops (S n) (@gReifiers_cons n sR1 rs))
+       (@inR_subEff (S n) sR (@gReifiers_cons n sR1 rs)
+          {| inR_idx := 0%fin; inR_lookup := Heq |}) op).
+      generalize (subEff_opid op : opid (gReifiers_ops (gReifiers_cons sR1 rs))).
+      simpl reifiers_re.
+      destruct  as [op1|op1].
+    Set Printing All.
+
+      simpl.
+Eval simpl in . 
+      simpl reifiers_re.
+      unfold inR_conv_state.
+      simpl inR_conv_state.
+      simpl.
+
+      
+[F stateF re ? ?]
+    s
+    set fs1 := inR_conv_state rest σ.
+    refine (reifiers_re rs (subEff_opid op) X (ofe_iso_1 (subEff_ins op) i,fs1) = _).
+    refine (optionO_map _ (sReifier_re sR op X _ (i,σ))).
+    refine (prodO_map (ofe_iso_1 (subEff_outs op)) _).
+    apply (inR_conv_state rest).
+    Show Proof.
+    refine (_ ◎ _); last first.
+    + apply (sRs_transport (eq_sym inR_lookup)).
+    + refine (λne σ2, ofe_iso_1 (rs_state_decomp inR_idx rs) (σ2, rest)).
+      solve_proper.
+        Show Proof.
+      subR_reify (op : opid F) X `{Cofe X}
+        (i : Ins (F op) ♯ X) (s : stateF ♯ X) (s_rest : rest ♯ X) :
+        let i' := subEff_conv_ins i in
+        let s' := subState_conv_state s_rest s in
+        reifiers_re rs (subEff_opid op) X (i',s') ≡
+          optionO_map (prodO_map subEff_conv_outs (subState_conv_state s_rest))
+                      (re op X _ (i,s))
+
+               
+
+  Context {n : nat} (rs : gReifiers n).
+  Notation F := (gReifiers_ops rs).
+  Notation stateF := (gReifiers_state rs).
+  Notation IT := (IT F).
+  Notation ITV := (ITV F).
 
   Notation stateM := ((stateF ♯ IT -n> (stateF ♯ IT) * IT))%type.
   #[local] Instance stateT_inhab : Inhabited stateM.
@@ -87,20 +651,20 @@ Section reify.
     λne x s, (s, Tau $ laterO_map fstO x).
   Solve All Obligations with solve_proper.
 
-  Program Definition reify_vis ( op : opid E ) :
-   oFunctor_car (Ins (E op)) (sumO IT stateM) (prodO IT stateM) -n>
-     (oFunctor_car (Outs (E op)) (prodO IT stateM) (sumO IT stateM) -n> laterO (prodO IT stateM)) -n> stateM.
+  Program Definition reify_vis ( op : opid F ) :
+   oFunctor_car (Ins (F op)) (sumO IT stateM) (prodO IT stateM) -n>
+     (oFunctor_car (Outs (F op)) (prodO IT stateM) (sumO IT stateM) -n> laterO (prodO IT stateM)) -n> stateM.
   Proof.
     simpl.
     simple refine (λne i (k : _ -n> _) (s : stateF ♯ IT), _).
     - simple refine (let ns := reifiers_re rs op _ (oFunctor_map _ (inlO,fstO) i, s) in _).
       simple refine (from_option (λ ns,
-                         let out2' := k $ oFunctor_map (Outs (E op)) (fstO,inlO) ns.1 in
+                         let out2' := k $ oFunctor_map (Outs (F op)) (fstO,inlO) ns.1 in
                          (ns.2, Tau $ laterO_map fstO out2'))
                        (s, Err RuntimeErr) ns).
-    - intros n s1 s2 Hs. simpl. eapply (from_option_ne (dist n)); solve_proper.
-    - intros n k1 k2 Hk s. simpl. eapply (from_option_ne (dist n)); solve_proper.
-    - intros n i1 i2 Hi k s. simpl. eapply (from_option_ne (dist n)); solve_proper.
+    - intros m s1 s2 Hs. simpl. eapply (from_option_ne (dist m)); solve_proper.
+    - intros m k1 k2 Hk s. simpl. eapply (from_option_ne (dist m)); solve_proper.
+    - intros m i1 i2 Hi k s. simpl. eapply (from_option_ne (dist m)); solve_proper.
   Defined.
 
   Program Definition reify_err : errorO -n> stateM := λne e s, (s, Err e).
@@ -111,7 +675,7 @@ Section reify.
 
   Program Definition unr : stateM -n>
     sumO (sumO (sumO (sumO natO errorO) (laterO (stateM -n> stateM))) (laterO stateM))
-      (sigTO (λ op : opid E, prodO (oFunctor_apply (Ins (E op)) stateM) (oFunctor_apply (Outs (E op)) stateM -n> laterO stateM))).
+      (sigTO (λ op : opid F, prodO (oFunctor_apply (Ins (F op)) stateM) (oFunctor_apply (Outs (F op)) stateM -n> laterO stateM))).
   Proof. simple refine (λne d, inl (inl (inl (inr (RuntimeErr))))). Qed.
 
   Definition reify : IT -n> stateM
@@ -160,8 +724,8 @@ Section reify.
       apply IT_rec1_vis. }
     Opaque prod_in. simpl.
     pose (r := (reifiers_re rs op _
-      (oFunctor_map (Ins (E op)) (inlO, fstO)
-                    (oFunctor_map (Ins (E op)) (sumO_rec idfun unreify, prod_in idfun reify) i), σ))).
+      (oFunctor_map (Ins (F op)) (inlO, fstO)
+                    (oFunctor_map (Ins (F op)) (sumO_rec idfun unreify, prod_in idfun reify) i), σ))).
     fold r.
     assert (r ≡ reifiers_re rs op _ (i,σ)) as Hr'.
     { unfold r. f_equiv. f_equiv.
@@ -176,8 +740,8 @@ Section reify.
           (laterO_map fstO
              (laterO_map (prod_in idfun reify)
                 (k
-                   (oFunctor_map (Outs (E op)) (prod_in idfun reify, sumO_rec idfun unreify)
-                      (oFunctor_map (Outs (E op)) (fstO, inlO) ns.1)))))))
+                   (oFunctor_map (Outs (F op)) (prod_in idfun reify, sumO_rec idfun unreify)
+                      (oFunctor_map (Outs (F op)) (fstO, inlO) ns.1)))))))
              (σ, Err RuntimeErr) (Some (o,σ'))).
     { apply from_option_proper; solve_proper. }
     simpl. repeat f_equiv.
@@ -203,8 +767,8 @@ Section reify.
       apply IT_rec1_vis. }
     simpl.
     pose (r := (reifiers_re rs op _
-      (oFunctor_map (Ins (E op)) (inlO, fstO)
-                    (oFunctor_map (Ins (E op)) (sumO_rec idfun unreify, prod_in idfun reify) i), σ))).
+      (oFunctor_map (Ins (F op)) (inlO, fstO)
+                    (oFunctor_map (Ins (F op)) (sumO_rec idfun unreify, prod_in idfun reify) i), σ))).
     fold r.
     assert (r ≡ reifiers_re rs op _ (i,σ)) as Hr'.
     { unfold r. f_equiv. f_equiv.
@@ -219,8 +783,8 @@ Section reify.
           (laterO_map fstO
              (laterO_map (prod_in idfun reify)
                 (k
-                   (oFunctor_map (Outs (E op)) (prod_in idfun reify, sumO_rec idfun unreify)
-                      (oFunctor_map (Outs (E op)) (fstO, inlO) ns.1)))))))
+                   (oFunctor_map (Outs (F op)) (prod_in idfun reify, sumO_rec idfun unreify)
+                      (oFunctor_map (Outs (F op)) (fstO, inlO) ns.1)))))))
              (σ, Err RuntimeErr) None).
     { apply from_option_proper; solve_proper. }
     reflexivity.
@@ -296,7 +860,9 @@ Section reify.
   Qed.
 
 End reify.
-Arguments reify {E} rs.
+Arguments reify {n} rs.
+
+
 
 Class subState {E : opsInterp}
   (stateF : oFunctor) (rs : reifiers E) (rest : oFunctor) :=
